ex2/imp_org.v
@@ -1,0 +1,115 @@
+Set Implicit Arguments.
+
+
+Inductive var := a | b | n | x | y.
+
+Definition op := nat -> nat -> nat.
+  
+Inductive expr :=
+  expr_var : var -> expr
+| expr_num : nat -> expr
+| expr_op : expr -> op -> expr -> expr.
+
+Inductive cmd :=
+  assign : var -> expr -> cmd
+| seq : cmd -> cmd -> cmd
+| skip : cmd
+| if_then_else : expr -> cmd -> cmd -> cmd
+| while : expr -> cmd -> cmd
+| assume : expr -> cmd.
+
+Definition state := var -> nat.
+
+Fixpoint sem (e : expr) (s : state) :=
+  match e with
+  | expr_var v => s v
+  | expr_num m => m
+  | expr_op e1 op e2 => op (sem e1 s) (sem e2 s)
+  end.
+
+
+(* -- Defining the program `euclid` in IMP -- *)
+Require Import Arith.
+Require Import Lia.
+Import Nat.
+
+(* some operators *)
+Definition gt01 n m := if gt_dec n m then 1 else 0.
+Definition ne01 n m := if eq_dec n m then 0 else 1.
+
+(* This notation will shorten things a bit *)
+Notation "$ v" := (expr_var v) (at level 7, format "$ v").
+
+Definition euclid_body :=
+    seq (assume (expr_op $a ne01 $b))
+        (if_then_else (expr_op $a gt01 $b)
+                      (assign a (expr_op $a sub $b))
+                      (assign b (expr_op $b sub $a))).
+
+(* copy pasted GCD definition from euclid.v - Nat does not work here *)
+Inductive gcd : nat -> nat -> nat -> Prop :=
+  base   : forall z, gcd z z z
+| step_a : forall a b z, gcd a b z -> gcd (a + b) b z
+| step_b : forall a b z, gcd a b z -> gcd a (a + b) z.
+
+(* copy pasted the tc tc' definitions *)
+Section ReflexiveTransitiveClosureAltDef.
+
+  Variable D : Set.
+  Variable R : D -> D -> Prop.
+
+  Inductive tc' : D -> D -> Prop :=
+    tc'_refl : forall s, tc' s s
+  | tc'_step : forall s u t, R s u -> tc' u t -> tc' s t.
+
+End ReflexiveTransitiveClosureAltDef.
+
+Section ReflexiveTransitiveClosureDef.
+
+  Variable D : Set.
+  Variable R : D -> D -> Prop.
+
+  Inductive tc : D -> D -> Prop :=
+    tc_refl : forall s, tc s s
+  | tc_step : forall s u t, tc s u -> R u t -> tc s t.
+
+End ReflexiveTransitiveClosureDef.
+
+Definition eq_var_dec : forall (v1 v2 : var), {v1 = v2} + {v1 <> v2}.
+Proof. decide equality. Qed.
+
+Definition update (st : state) (v : var) (n : nat) : state :=
+  fun x => if eq_var_dec x v then n else st x.
+
+Inductive sos : (state * cmd) -> (state * cmd) -> Prop := 
+  | step_seq : forall st c1 st' c1' c2, 
+    sos (st, c1) (st', c1') -> sos (st, seq c1 c2) (st', seq c1' c2)
+  | step_seq_skip : forall st c2, 
+    sos (st, seq skip c2) (st, c2)
+  | step_assign : forall st v e, 
+    sos (st, assign v e) (update st v (sem e st), skip)
+  | step_if_true : forall st e c1 c2, 
+    sem e st <> 0 -> sos (st, if_then_else e c1 c2) (st, c1)
+  | step_if_false : forall st e c1 c2, 
+    sem e st = 0 -> sos (st, if_then_else e c1 c2) (st, c2)
+  | step_while_true : forall st e c, 
+    sem e st <> 0 -> sos (st, while e c) (st, seq c (while e c))
+  | step_while_false : forall st e c, 
+    sem e st = 0 -> sos (st, while e c) (st, skip)
+  | step_assume_true : forall st e, 
+    sem e st <> 0 -> sos (st, assume e) (st, skip).
+ 
+Inductive step : state -> state -> Prop := 
+  | cons : forall st st', sos (st, euclid_body) (st', skip) -> step st st'.
+  
+Lemma Q4 : forall a0 b0 s s', s a = a0 -> s b = b0 -> tc' step s s' -> s' a = s' b -> gcd a0 b0 (s' a).
+Proof.
+  intros a0 b0 s s' Ha0 Hb0 Hstepss Hskip.
+  induction Hstepss.
+  - assert (Heq : a0 = b0) by lia.
+    rewrite Ha0.
+    rewrite Heq.
+    apply base.
+  - inversion H.
+    inversion H0.
+Qed.
